user 3, session 11016, part 26

diffs-annotated/3/user-3-session-11016.v
@@ -242,14 +242,37 @@ Qed.
 Fixpoint count (v : nat) (s : bag) : nat :=
   match s with
   | [ ] => 0
-  | x :: s' => (if beq_nat x v then 1 else 0) + count v s'
+  | x :: s => (if beq_nat x v then 1 else 0) + count v s
   end.
-Redirect "/var/folders/5x/1mdbpbjd7012l971fq0zkj2w0000gn/T/coqPj8Aul"
+Redirect "/var/folders/5x/1mdbpbjd7012l971fq0zkj2w0000gn/T/coqZJhIxJ"
 Print Ltac Signatures.
 Timeout 1 Print Grammar tactic.
 Add Search Blacklist "Raw" "Proofs".
 Set Search Output Name Only.
-Redirect "/var/folders/5x/1mdbpbjd7012l971fq0zkj2w0000gn/T/coqjyWfCR"
+Redirect "/var/folders/5x/1mdbpbjd7012l971fq0zkj2w0000gn/T/coqmV969N"
 SearchPattern _.
 Remove Search Blacklist "Raw" "Proofs".
 Unset Search Output Name Only.
+Example test_count1 : count 1 [1; 2; 3; 1; 4; 1] = 3.
+Proof.
+reflexivity.
+Qed.
+Example test_count2 : count 6 [1; 2; 3; 1; 4; 1] = 0.
+Proof.
+reflexivity.
+Qed.
+Definition sum : bag -> bag -> bag := app.
+Redirect "/var/folders/5x/1mdbpbjd7012l971fq0zkj2w0000gn/T/coqJaAeme"
+Print Ltac Signatures.
+Timeout 1 Print Grammar tactic.
+Add Search Blacklist "Raw" "Proofs".
+Set Search Output Name Only.
+Redirect "/var/folders/5x/1mdbpbjd7012l971fq0zkj2w0000gn/T/coqxgre7c"
+SearchPattern _.
+Remove Search Blacklist "Raw" "Proofs".
+Unset Search Output Name Only.
+Example test_sum1 : count 1 (sum [1; 2; 3] [1; 4; 1]) = 3.
+Proof.
+reflexivity.
+QEd.
+(* Failed. *)
